refactor

paxos/proof.dfy
@@ -44,8 +44,11 @@ predicate Validity_Inv(c:Constants, ds:DistrSys, v:Value)
     && Validity_Inv_AllMessegesContainV(c, ds, v)
 }
 
-predicate Validity_Inv_AllMessegesContainV(c:Constants, ds:DistrSys, v:Value) {
-    forall pkt | pkt in ds.network.sentPackets :: MessageContainsV(pkt.msg, v)
+predicate Validity_Inv_AllMessegesContainV(c:Constants, ds:DistrSys, v:Value) 
+    requires c.WF()
+    requires ds.WF(c)
+{
+    AllProcessesInitV(c, ds, v) ==> forall pkt | pkt in ds.network.sentPackets :: MessageContainsV(pkt.msg, v)
 }
 
 predicate MessageContainsV(m: Message, v:Value) {
@@ -62,21 +65,20 @@ predicate Validity_Inv_AllAccAcceptsV(c:Constants, ds:DistrSys, v:Value)
     requires c.WF()
     requires ds.WF(c)
 {
-    forall i | c.ValidAccIdx(i) :: ds.acceptors[i].accepted != v ==> ds.acceptors[i].accepted == Nil 
+    AllProcessesInitV(c, ds, v) ==> forall i | c.ValidAccIdx(i) :: ds.acceptors[i].accepted != v ==> ds.acceptors[i].accepted == Nil 
 }
 
 predicate Validity_Inv_AllLdrProposeV(c:Constants, ds:DistrSys, v:Value)
     requires c.WF()
     requires ds.WF(c)
 {
-    forall i | c.ValidLdrIdx(i) :: ds.leaders[i].val == v
+    AllProcessesInitV(c, ds, v) ==> forall i | c.ValidLdrIdx(i) :: ds.leaders[i].val == v
 }
 
 
 /* Init ==>  Validity_Inv */
 lemma InitImpliesInv(c:Constants, ds:DistrSys, v:Value) 
     requires Init(c, ds)
-    requires AllProcessesInitV(c, ds, v)
     ensures Validity_Inv(c, ds, v)
 {}
 
@@ -84,7 +86,6 @@ lemma InitImpliesInv(c:Constants, ds:DistrSys, v:Value)
 /* Validity_Inv && Next ==>  Validity_Inv' */
 lemma NextPreservesInv(c:Constants, v:Value, ds:DistrSys, ds':DistrSys) 
     requires Validity_Inv(c, ds, v)
-    requires AllProcessesInitV(c, ds, v)
     requires Next(c, ds, ds')
     ensures Validity_Inv(c, ds', v)
 {}
